cleanup translation in axiomatic glueing; wip

theories/axiomatic.v
@@ -1,5 +1,5 @@
 (* a rough sketch of a glueing of the thread-local semantics of isla with an axiomatic memory model *)
-(* has fetching, but no mixed-size, no page tables, and does not treat system registers properly *)
+(* has fetching, partial page tables (single level, no faults), but no mixed-size, and does not treat system registers properly *)
 (* TODO: this really needs proof-reading *)
 
 (* TODO: how to test this given that it produces infinite things, and is very not computing?
@@ -7,8 +7,7 @@ Maybe make an "up to n steps" version and prove some relation? *)
 
 (* TODO: there is a design flaw with our encoding of pre-executions that forces having infinitely many initial events  *)
 
-Require Import isla.base.
-Require Import isla.opsem.
+Require Import isla.base isla.opsem.
 
 From RecordUpdate Require Import RecordSet.
 Import RecordSetNotations.
@@ -17,26 +16,27 @@ Definition thread_internal_event_id := nat.
 Definition thread_id := nat.
 Definition event_id := (thread_id * thread_internal_event_id)%type.
 
-Inductive memory_action :=
-| Act (a:trace_label)
+Inductive translation_stage : Type :=
+| Tstg_stage1
+| Tstg_stage2.
+
+Inductive memory_action : Type :=
+| MA_act (a:trace_label)
   (* TODO: we use these for now, but
   (1) they have to change, e.g. they don't currently have barriers, and
   (2) the interface between isla-coq and the memory model itself feels wrong
   *)
-| Fetch (a:addr) (v:valu)
-| Translate1 (va:addr) (ipa:addr)
-| Translate2 (ipa:addr) (pa:addr).
+| MA_fetch (a:addr) (v:valu)
+| MA_translate (stg:translation_stage) (hi:addr) (lo_opt:option addr).
+
+Definition rel := event_id -> event_id -> Prop.
 
 Record pre_execution := {
   (* The number of threads in the pre-execution *)
   pe_threads : nat; (* TODO: make the memory model ignore events over that tid *)
   (* the labelling function, labelling each event with its memory actions *)
   pe_label : event_id -> memory_action; (* TODO: or option? *)
-  (* The fetch-to-execute order relates a fetch to the event it fetches for:
-    F x v --fe--> R x v', where decode(v) = R x
-  *)
-  pe_fe : event_id -> event_id -> Prop;
-  (* The transitive reduction (because it's easier to compute) of `fpo`, the analogue pf program-order for `Fetch` events
+  (* Fetch program order, the analogue of program-order for `Fetch` events
   Instead of a primitive `po` between `b` and `d`, we have
     a:F x1 v1 -------> b:A1
        |               .
@@ -45,20 +45,21 @@ Record pre_execution := {
        v               v
     c:F x2 v2 -------> d:A2
   *)
-  pe_fpo1 : event_id -> event_id -> Prop;
-  (* data dependencies.
+  pe_fpo : rel;
+  (** data dependencies.
     `r = R x; W y r` leads to
-       R x v --data--> W y v
+    R x v --data--> W y v
   *)
-  pe_data : event_id -> event_id -> Prop;
-  (* address dependencies *)
-  pe_addr : event_id -> event_id -> Prop;
-  (* translation data dependencies (correspond to address dependencies) *)
-  pe_tdata : event_id -> event_id -> Prop;
-  (* control dependencies *)
-  pe_ctrl : event_id -> event_id -> Prop;
-  (* intra-instruction ordering: T1 --iio--> T2 --iio--> W *)
-  pe_iio : event_id -> event_id -> Prop;
+  pe_data : rel;
+  (** address dependencies *)
+  pe_addr : rel;
+  (** translation data dependencies (correspond to address dependencies) *)
+  pe_tdata : rel;
+  (** control dependencies *)
+  pe_ctrl : rel;
+  (** intra-instruction order: F --iio--> T1 --iio--> T2 --iio--> [R|W] *)
+  pe_iio : rel;
+  (* TODO: others??? *)
 }.
 
 (** TODO: *)
@@ -72,8 +73,8 @@ Record dependency_info := {
 (* TODO: not clear how to deal with this *)
 Axiom decode : valu -> (dependency_info * list trc).
 
-(** instrumented register map, where a register is mapped to the events that it "depends" on *)
-Definition instrumented_reg_map := gmap string (thread_internal_event_id -> Prop).
+(** dependency_reg_map register map, where a register is mapped to the events that it "depends" on *)
+Definition dependency_reg_map := gmap string (thread_internal_event_id -> Prop).
 
 Inductive translation_level : Type :=
 (* TODO: it's probably more complicated *)
@@ -85,41 +86,44 @@ Inductive translation_level : Type :=
 (** accumulator to build a pre-execution *)
 Record info := mk_info {
   info_tr : trc;
-  info_regs : instrumented_reg_map;
-  info_regs2 : reg_map;
-  info_cur_eid : thread_internal_event_id;
-  info_fe_src : thread_internal_event_id;
+  info_register_dependencies : dependency_reg_map;
+  info_registers : reg_map;
+  info_current_eid : thread_internal_event_id;
+  info_current_fetch : thread_internal_event_id;
+  info_fe_srcs : thread_internal_event_id -> Prop;
   info_ctrl_srcs : thread_internal_event_id -> Prop;
   info_data_srcs : thread_internal_event_id -> Prop;
   info_addr_srcs : thread_internal_event_id -> Prop;
   info_translation_level : translation_level;
-  (* TODO:
+  (* TODO: ???
   info_address_announced : bool;
   *)
-  (* TODO: iio? *)
 }.
 
 Instance eta_info : Settable _ :=
-  settable! mk_info <info_tr;
-    info_regs;
-    info_regs2;
-    info_cur_eid;
-    info_fe_src;
+  settable! mk_info <
+    info_tr;
+    info_register_dependencies;
+    info_registers;
+    info_current_eid;
+    info_current_fetch;
+    info_fe_srcs;
     info_ctrl_srcs;
     info_data_srcs;
     info_addr_srcs;
     info_translation_level>.
 
 Definition info_agrees (info1 info2 : info) : Prop :=
-  info1 = info2. (* TODO: should probably require equal extensions *)
+  (* TODO: should probably require equal extensions *)
+  info1 = info2.
 
-Definition event_deps_of_reg_deps (reg_deps : string -> Prop) (info_regs : instrumented_reg_map) (le : thread_internal_event_id) : Prop :=
+Definition event_deps_of_reg_deps (reg_deps : string -> Prop) (info_regs : dependency_reg_map) (le : thread_internal_event_id) : Prop :=
   exists r s,
     reg_deps r /\
     info_regs !! r = Some s /\
     s le.
 
-Definition update_regs (updated_registers : string -> Prop) (le : thread_internal_event_id) (iregs : instrumented_reg_map) (iregs' : instrumented_reg_map) : Prop :=
+Definition update_regs (updated_registers : string -> Prop) (le : thread_internal_event_id) (iregs : dependency_reg_map) (iregs' : dependency_reg_map) : Prop :=
   forall r,
     (updated_registers r ->
       match iregs' !! r with
@@ -134,30 +138,40 @@ Definition update_regs (updated_registers : string -> Prop) (le : thread_interna
       | None, None => True
       end).
 
-Definition regs_empty (iregs : instrumented_reg_map) : Prop :=
+Definition regs_empty (iregs : dependency_reg_map) : Prop :=
   forall r,
     match iregs !! r with
     | None => True
     | Some s => forall le, ~ s le
     end.
 
-Definition pre_execution_of_fetch is_initial addr tid pe Xnow Xfuture : Prop :=
-  let e := (tid, Xnow.(info_cur_eid)) in
+Definition pre_execution_of_fetch addr tid pe Xnow Xfuture : Prop :=
+  let e := (tid, Xnow.(info_current_eid)) in
   exists v tr' regs',
-    pe.(pe_label) e = Fetch addr v /\
+    pe.(pe_label) e = MA_fetch addr v /\
     let (depinfo, trs) := decode v in
     List.In tr' trs /\
-    update_regs depinfo.(depinfo_regs_out) Xnow.(info_cur_eid) Xnow.(info_regs) regs' /\
+    update_regs depinfo.(depinfo_regs_out) Xnow.(info_current_eid) Xnow.(info_register_dependencies) regs' /\
     let Xnext := Xnow <| info_tr := tr' |>
-      <| info_cur_eid := (Xnow.(info_cur_eid) + 1)%nat |>
-      <| info_fe_src := Xnow.(info_cur_eid) |>
-      <| info_ctrl_srcs := (fun le => Xnow.(info_ctrl_srcs) le \/ (depinfo.(depinfo_is_ctrl) /\ le = Xnow.(info_cur_eid))) |>
-      <| info_data_srcs := event_deps_of_reg_deps depinfo.(depinfo_regs_in_data) Xnow.(info_regs) |>
-      <| info_addr_srcs := event_deps_of_reg_deps depinfo.(depinfo_regs_in_addr) Xnow.(info_regs) |>
-      <| info_regs := regs' |> in
-    (~ is_initial -> pe.(pe_fpo1) (tid, Xnow.(info_fe_src)) e) /\
-    (forall e', pe.(pe_fpo1) e' (tid, Xnow.(info_cur_eid)) -> e' = (tid, Xnow.(info_fe_src) )) /\
+      <| info_current_eid := (Xnow.(info_current_eid) + 1)%nat |>
+      <| info_current_fetch := Xnow.(info_current_eid) |>
+      <| info_fe_srcs := (fun le => Xnow.(info_fe_srcs) le \/ le = Xnow.(info_current_eid)) |>
+      <| info_ctrl_srcs := (fun le => Xnow.(info_ctrl_srcs) le \/ (depinfo.(depinfo_is_ctrl) /\ le = Xnow.(info_current_eid))) |>
+      <| info_data_srcs := event_deps_of_reg_deps depinfo.(depinfo_regs_in_data) Xnow.(info_register_dependencies) |>
+      <| info_addr_srcs := event_deps_of_reg_deps depinfo.(depinfo_regs_in_addr) Xnow.(info_register_dependencies) |>
+      <| info_register_dependencies := regs' |> in
+    (* fpo *)
+    (forall le', Xnow.(info_fe_srcs) le' -> pe.(pe_fpo) (tid, le') e) /\
+    (forall e', pe.(pe_fpo) e' (tid, Xnow.(info_current_eid)) -> exists le', e' = (tid, le') /\ Xnow.(info_fe_srcs) le') /\
+    (* ctrl *)
     (~ (exists e', pe.(pe_ctrl) e' e)) /\
+    (* addr *)
+    (~ (exists e', pe.(pe_addr) e' e)) /\
+    (* data *)
+    (~ (exists e', pe.(pe_data) e' e)) /\
+    (* tdata *)
+    (~ (exists e', pe.(pe_tdata) e' e)) /\
+    (* TODO: others? *)
     info_agrees Xnext Xfuture.
 
 Definition replace_addr (a:trace_label) (x:addr) : trace_label :=
@@ -186,10 +200,10 @@ Definition pre_execution_of_memory_action tid pe a tr' Xnow Xfuture : Prop :=
   | None => False
   | Some addr =>
   let k := (match Xnow.(info_translation_level) with | Trlvl_plain_address => 0 | Trlvl_translation_off => 0 | Trlvl_stage_one_only => 1 | Trlvl_stage_one_and_two => 2 end)%nat in
-  let e := (tid, Xnow.(info_cur_eid) + k)%nat in
+  let e := (tid, Xnow.(info_current_eid) + k)%nat in
   (match Xnow.(info_translation_level) with
   | Trlvl_plain_address =>
-    pe.(pe_label) e = Act a /\
+    pe.(pe_label) e = MA_act a /\
     (forall e', Xnow.(info_addr_srcs) e' -> (tid, e') <> e -> pe.(pe_addr) (tid, e') e) /\
     (* addr *)
     (forall e', Xnow.(info_addr_srcs) e' -> (tid, e') <> e -> pe.(pe_addr) (tid, e') e) /\
@@ -197,25 +211,31 @@ Definition pre_execution_of_memory_action tid pe a tr' Xnow Xfuture : Prop :=
     (* tdata *)
     (forall e', ~ pe.(pe_tdata) e' e) /\
     (* iio *)
-    (forall e', ~ pe.(pe_iio) e' e) /\
+    pe.(pe_iio) (tid, Xnow.(info_current_fetch)) e /\
+    (forall e', pe.(pe_iio) e' e -> e' = (tid, Xnow.(info_current_fetch))) /\
+    (* fpo *)
+    (forall e', ~ pe.(pe_fpo) e' e) /\
     (* TODO: ??? *)
     True
   | Trlvl_translation_off =>
-    pe.(pe_label) e = Act a /\
+    pe.(pe_label) e = MA_act a /\
     (forall e', Xnow.(info_addr_srcs) e' -> (tid, e') <> e -> pe.(pe_addr) (tid, e') e) /\
     (* addr *)
     (forall e', ~ pe.(pe_addr) e' e) /\
     (* tdata *)
     (forall e', ~ pe.(pe_tdata) e' e) /\
     (* iio *)
-    (forall e', ~ pe.(pe_iio) e' e) /\
-    (* TODO: ??? *)
+    pe.(pe_iio) (tid, Xnow.(info_current_fetch)) e /\
+    (forall e', pe.(pe_iio) e' e -> e' = (tid, Xnow.(info_current_fetch))) /\
+    (* fpo *)
+    (forall e', ~ pe.(pe_fpo) e' e) /\
+    (* TODO *)
     True
   | Trlvl_stage_one_only =>
-    let etr := (tid, Xnow.(info_cur_eid)) in
+    let etr := (tid, Xnow.(info_current_eid)) in
     exists ipa,
-    pe.(pe_label) e = Act (replace_addr a ipa) /\
-    pe.(pe_label) etr = Translate1 addr ipa /\
+    pe.(pe_label) e = MA_act (replace_addr a ipa) /\
+    pe.(pe_label) etr = MA_translate Tstg_stage1 addr (Some ipa) /\
     (* addr *)
     (forall e', ~ pe.(pe_addr) e' e) /\
     (forall e', ~ pe.(pe_addr) e' etr) /\
@@ -224,17 +244,21 @@ Definition pre_execution_of_memory_action tid pe a tr' Xnow Xfuture : Prop :=
     (forall e', pe.(pe_tdata) e' etr -> exists le', Xnow.(info_addr_srcs) le' /\ e' = (tid, le') /\ e' <> etr) /\
     (forall e', ~ pe.(pe_tdata) e' e) /\
     (* iio *)
-    (forall e', ~ pe.(pe_iio) e' etr) /\
-    (pe.(pe_iio) etr e) /\
-    (forall e', pe.(pe_iio) e' e -> e' = etr) /\
-    True (* TODO *)
+    pe.(pe_iio) (tid, Xnow.(info_current_fetch)) etr /\
+    pe.(pe_iio) (tid, Xnow.(info_current_fetch)) e /\
+    pe.(pe_iio) etr e /\
+    (forall e', pe.(pe_iio) e' etr -> e' = (tid, Xnow.(info_current_fetch))) /\
+    (forall e', pe.(pe_iio) e' e -> e' = (tid, Xnow.(info_current_fetch)) \/ e' = etr) /\
+    (* fpo *)
+    (forall e', ~ pe.(pe_fpo) e' e) /\
+    True (* TODO: tpo, ... *)
   | Trlvl_stage_one_and_two =>
-    let etr1 := (tid, Xnow.(info_cur_eid)) in
-    let etr2 := (tid, Xnow.(info_cur_eid) + 1)%nat in
+    let etr1 := (tid, Xnow.(info_current_eid)) in
+    let etr2 := (tid, Xnow.(info_current_eid) + 1)%nat in
     exists ipa pa,
-    pe.(pe_label) e = Act (replace_addr a pa) /\
-    pe.(pe_label) etr1 = Translate1 addr ipa /\
-    pe.(pe_label) etr2 = Translate2 ipa pa /\
+    pe.(pe_label) e = MA_act (replace_addr a pa) /\
+    pe.(pe_label) etr1 = MA_translate Tstg_stage1 addr (Some ipa) /\
+    pe.(pe_label) etr2 = MA_translate Tstg_stage2 ipa (Some pa) /\
     (* addr *)
     (forall e', ~ pe.(pe_addr) e' e) /\
     (forall e', ~ pe.(pe_addr) e' etr1) /\
@@ -245,19 +269,21 @@ Definition pre_execution_of_memory_action tid pe a tr' Xnow Xfuture : Prop :=
     (forall e', ~ pe.(pe_tdata) e' etr2) /\
     (forall e', ~ pe.(pe_tdata) e' e) /\
     (* iio *)
-    (forall e', ~ pe.(pe_iio) e' etr1) /\
-    (pe.(pe_iio) etr1 etr2) /\
-    (pe.(pe_iio) etr2 e) /\
-    (pe.(pe_iio) etr1 e) /\
-    (forall e', pe.(pe_iio) e' e -> e' = etr1 \/ e' = etr2) /\
-    (forall e', pe.(pe_iio) e' etr2 -> e' = etr1) /\
-    True (* TODO *)
+    pe.(pe_iio) (tid, Xnow.(info_current_fetch)) etr1 /\
+    pe.(pe_iio) (tid, Xnow.(info_current_fetch)) etr2 /\
+    pe.(pe_iio) (tid, Xnow.(info_current_fetch)) e /\
+    pe.(pe_iio) etr1 etr2 /\
+    pe.(pe_iio) etr1 e /\
+    pe.(pe_iio) etr2 e /\
+    (forall e', pe.(pe_iio) e' etr1 -> e' = (tid, Xnow.(info_current_fetch))) /\
+    (forall e', pe.(pe_iio) e' etr2 -> e' = etr1 \/ e' = (tid, Xnow.(info_current_fetch))) /\
+    (forall e', pe.(pe_iio) e' e -> e' = (tid, Xnow.(info_current_fetch)) \/ e' = etr1 \/ e' = etr2) /\
+    (* fpo *)
+    (forall e', ~ pe.(pe_fpo) e' e) /\
+    True (* TODO: ??? *)
   end) /\
   let Xnext := Xnow <| info_tr := tr' |>
-    <| info_cur_eid := (Xnow.(info_cur_eid) + 1 + k)%nat |> in
-  (* fe *)
-  pe.(pe_fe) (tid, Xnow.(info_fe_src)) e /\
-  (forall e', pe.(pe_fe) e' e -> e' = (tid, Xnow.(info_fe_src) )) /\
+    <| info_current_eid := (Xnow.(info_current_eid) + 1 + k)%nat |> in
   (* ctrl *)
   (forall e', Xnow.(info_ctrl_srcs) e' -> (tid, e') <> e -> pe.(pe_ctrl) (tid, e') e) /\
   (forall e', pe.(pe_ctrl) e' e -> e' <> e /\ exists le', Xnow.(info_ctrl_srcs) le' /\ e' = (tid, le')) /\
@@ -277,18 +303,19 @@ Record thread_state := {
 Definition pre_execution_of_thread (tid : thread_id) (regs : thread_state) (pe : pre_execution) : Prop :=
   exists (X : nat -> info),
   (X (0%nat)).(info_tr) = [] /\
-  regs_empty (X (0%nat)).(info_regs) /\
-  (X (0%nat)).(info_regs2) = regs.(ts_regs) /\
+  regs_empty (X (0%nat)).(info_register_dependencies) /\
+  (X (0%nat)).(info_registers) = regs.(ts_regs) /\
   (X (0%nat)).(info_translation_level) = regs.(ts_translation_level) /\
   (forall e, ~ (X (0%nat)).(info_ctrl_srcs) e) /\
+  (forall e, ~ (X (0%nat)).(info_fe_srcs) e) /\
   forall (n : nat),
   let Xnow := X n in
   match Xnow.(info_tr) with
   | [] =>
-    match next_pc Xnow.(info_regs2) (* TODO: does this function do what I think it does? *) with
+    match next_pc Xnow.(info_registers) (* TODO: does this function do what I think it does? *) with
     | None => False (* TODO: what does this correspond to? *)
     | Some (addr, _) =>
-      pre_execution_of_fetch (n > 0) addr tid pe Xnow (X (n+1)%nat)
+      pre_execution_of_fetch addr tid pe Xnow (X (n+1)%nat)
     end
   | tr =>
     exists ao tr',
@@ -301,12 +328,12 @@ Definition pre_execution_of_thread (tid : thread_id) (regs : thread_state) (pe :
         let Xnext := Xnow <| info_tr := tr' |> in
         info_agrees Xnext (X (n+1)%nat)
       | Some (LReadReg r _ v) =>
-        Xnow.(info_regs2) !! r = Some v (* TODO: ? *) /\
+        Xnow.(info_registers) !! r = Some v (* TODO: ? *) /\
         let Xnext := Xnow <| info_tr := tr' |> in
         info_agrees Xnext (X (n+1)%nat)
       | Some (LWriteReg r _ v) =>
         let Xnext := Xnow <| info_tr := tr' |>
-         <| info_regs2 := (<[ r := v ]> Xnow.(info_regs2)) |> in
+         <| info_registers := (<[ r := v ]> Xnow.(info_registers)) |> in
         info_agrees Xnext (X (n+1)%nat)
       | Some (LReadMem _ _ _ _ _ as a | LWriteMem _ _ _ _ _ _ as a) =>
         pre_execution_of_memory_action tid pe a tr' Xnow (X (n+1)%nat)
@@ -333,21 +360,21 @@ Record memory_model := {
 
 Require Import Coq.Relations.Relation_Operators.
 
-Definition acyclic (r : event_id -> event_id -> Prop) : Prop :=
+Definition acyclic (r : rel) : Prop :=
   Irreflexive (clos_trans _ r).
 
-Definition does_not_involve_initial_events (pe : pre_execution) (R : event_id -> event_id -> Prop) : Prop :=
-  (forall e e', R e e' -> fst e <> 0 /\ fst e' <> 0)%nat.
+Definition does_not_involve_initial_events (pe : pre_execution) (r : rel) : Prop :=
+  (forall e e', r e e' -> fst e <> 0 /\ fst e' <> 0)%nat.
 
 (** `rf` is right-total on reads, and relates a write to a read when the read reads from the write, in which case they are at the same location and of the same value*)
-Definition wf_rf (pe : pre_execution) (rf : event_id -> event_id -> Prop) :=
+Definition wf_rf (pe : pre_execution) (rf : rel) :=
   does_not_involve_initial_events pe rf /\
   (forall e, (fst e <= pe.(pe_threads))%nat ->
     match pe.(pe_label) e with
-    | Act (LReadMem v _ addr _ _) =>
+    | MA_act (LReadMem v _ addr _ _) =>
       (exists w, rf w e /\
         match pe.(pe_label) e with
-        | Act (LWriteMem _ _ addr' v' _ _) => addr = addr' /\ v = v'
+        | MA_act (LWriteMem _ _ addr' v' _ _) => addr = addr' /\ v = v'
         | _ => False
         end) /\
       (forall w1 w2, rf w1 e -> rf w2 e -> w1 = w2)
@@ -355,14 +382,14 @@ Definition wf_rf (pe : pre_execution) (rf : event_id -> event_id -> Prop) :=
     end).
 
 (** `irf` is right-total on fetches, and relates a write to a fetch when the fetch reads from the write, in which case they are at the same location and of the same value*)
-Definition wf_irf (pe : pre_execution) (irf : event_id -> event_id -> Prop) : Prop :=
+Definition wf_irf (pe : pre_execution) (irf : rel) : Prop :=
   does_not_involve_initial_events pe irf /\
   (forall e, (fst e <= pe.(pe_threads))%nat ->
     match pe.(pe_label) e with
-    | Fetch addr v =>
+    | MA_fetch addr v =>
       (exists w, irf w e /\
         match pe.(pe_label) e with
-        | Act (LWriteMem _ _ addr' v' _ _) => addr' = Val_Bits (BVN 64 addr) /\ v = v'
+        | MA_act (LWriteMem _ _ addr' v' _ _) => addr' = Val_Bits (BVN 64 addr) /\ v = v'
         | _ => False
         end) /\
       (forall w1 w2, irf w1 e -> irf w2 e -> w1 = w2)
@@ -370,13 +397,13 @@ Definition wf_irf (pe : pre_execution) (irf : event_id -> event_id -> Prop) : Pr
     end).
 
 (** `co` is a per-location-total order over writes *)
-Definition wf_co (pe : pre_execution) (co : event_id -> event_id -> Prop) : Prop :=
+Definition wf_co (pe : pre_execution) (co : rel) : Prop :=
   (* initial events are always at the start of `co` *)
   (forall e tid e', co e (tid, e') -> tid <> 0%nat) /\
   (* writes at the same location are `co`-related *)
   (forall e e', (fst e <= pe.(pe_threads))%nat -> (fst e' <= pe.(pe_threads))%nat -> e <> e' ->
     match pe.(pe_label) e, pe.(pe_label) e' with
-    | Act (LWriteMem _ _ addr1 _ _ _), Act (LWriteMem _ _ addr2 _ _ _) =>
+    | MA_act (LWriteMem _ _ addr1 _ _ _), MA_act (LWriteMem _ _ addr2 _ _ _) =>
       addr1 = addr2 -> co e e' \/ co e' e
     | _, _ => False
     end) /\
@@ -384,14 +411,28 @@ Definition wf_co (pe : pre_execution) (co : event_id -> event_id -> Prop) : Prop
   (forall e e',
      co e e' ->
      match pe.(pe_label) e, pe.(pe_label) e' with
-     | Act (LWriteMem _ _ addr1 _ _ _), Act (LWriteMem _ _ addr2 _ _ _) => addr1 = addr2
+     | MA_act (LWriteMem _ _ addr1 _ _ _), MA_act (LWriteMem _ _ addr2 _ _ _) => addr1 = addr2
      | _, _ => False
      end) /\
   Transitive co /\
   Irreflexive co.
 
-(*** Sequential Consistency with Fetches, axiomatically
-     This requires translation being turned off. *)
+Definition is_fetch (pe : pre_execution) (e : event_id) : bool :=
+  match pe.(pe_label) e with
+  | MA_act _ => false
+  | MA_fetch _ _ => true
+  | MA_translate _ _ _ => false
+  end.
+
+Definition is_explicit_event (pe : pre_execution) (e : event_id) : bool :=
+  match pe.(pe_label) e with
+  | MA_act _ => true
+  | MA_fetch _ _ => false
+  | MA_translate _ _ _ => false
+  end.
+
+(** Sequential Consistency with Fetches, axiomatically
+    This requires translation being turned off. *)
 Definition sc : memory_model := {|
   mm_validity := (fun pe =>
   exists co rf irf,
@@ -399,15 +440,15 @@ Definition sc : memory_model := {|
   wf_irf pe irf /\
   wf_co pe co /\
   let fr := (fun r w => exists w0, rf w0 r /\ co w0 w) in
-  let fpo := (fun a b => clos_trans _ pe.(pe_fpo1) a b) in
-  let po := (fun a b => exists fa fb, pe.(pe_fe) fa a /\ pe.(pe_fe) fb b /\ fpo fa fb) in
-  let po_fetch0 := (fun a fb => exists b, po a b /\ pe.(pe_fe) fb b) in
-  let po_fetch := (fun a b => po_fetch0 a b \/ pe.(pe_fe) a b) in
+  let fe := (fun e1 e2 => pe.(pe_iio) e1 e2 /\ is_fetch pe e1 /\ is_explicit_event pe e2) in
+  let po := (fun a b => exists fa fb, fe fa a /\ fe fb b /\ pe.(pe_fpo) fa fb) in
+  let po_fetch0 := (fun a fb => exists b, po a b /\ fe fb b) in
+  let po_fetch := (fun a b => po_fetch0 a b \/ fe a b) in
   acyclic (fun a b => po a b \/ po_fetch a b \/ rf a b \/ fr a b \/ co a b)
   )
 |}.
 
-Definition either_way (r : event_id -> event_id -> Prop) (e1 e2 : event_id) : Prop :=
+Definition either_way (r : rel) (e1 e2 : event_id) : Prop :=
   r e1 e2 \/ r e2 e1.
 
 Definition initial_pre_execution_in (pe_initial_state pe : pre_execution) : Prop :=
@@ -418,8 +459,7 @@ Definition initial_pre_execution_in (pe_initial_state pe : pre_execution) : Prop
   (* no extraneous edges *)
   ~ (exists le e',
       let e := (0%nat, le) in
-      either_way pe.(pe_fe) e e' \/
-      either_way pe.(pe_fpo1) e e' \/
+      either_way pe.(pe_fpo) e e' \/
       either_way pe.(pe_data) e e' \/
       either_way pe.(pe_ctrl) e e' \/
       either_way pe.(pe_addr) e e' \/
@@ -427,7 +467,7 @@ Definition initial_pre_execution_in (pe_initial_state pe : pre_execution) : Prop
       either_way pe.(pe_iio) e e'
   ).
 
-(* TODO: need a way to specify `info` more, like translation level, etc. *)
+(** Top-level definition of the semantics of running a machine from a starting state `regss` *)
 Definition valid_execution_of (regss : list thread_state) (pe_initial_state : pre_execution) (pe : pre_execution) (mm : memory_model) : Prop :=
   initial_pre_execution_in pe_initial_state pe /\
   pre_execution_of_threads regss pe /\
